Testing new semantics

src/SemOp.v
@@ -5,484 +5,273 @@ Require Export SemanticsExprAction Semantics SemFacts.
 
 Set Implicit Arguments.
 
-Section GivenModule.
+Section BigSem.
   Variable m: Modules.
-  Variable oldRegs: RegsT.
+  Variable o: RegsT.
 
-  Inductive SemActionOp:
-    forall k, ActionT type k -> UpdatesT -> MethsT -> MethsT -> type k -> Prop :=
-  | SASMCallExt
+  Inductive SemActionBig:
+    forall k, ActionT type k -> list (SubstepRec m o) -> type k -> Prop :=
+  | SABMCassInt
+      meth body
+      (marg: Expr type (SyntaxKind (arg (projT1 body))))
+      (mret: type (ret (projT1 body)))
+      retK (fret: type retK)
+      (cont: type (ret (projT1 body)) -> ActionT type retK)
+      (HIn: In (meth :: body)%struct (getDefsBodies m))
+      css retv (HCont: SemActionBig (cont mret) css retv)
+      mss (HBig: SemActionBig (projT2 body type (evalExpr marg)) mss mret)
+      ul (Hul: ul = Meth (Some (meth :: (existT _ _ (evalExpr marg, mret)))%struct))
+      u cs (HSubstep: Substep m o u ul cs)
+      bss (Hbss: bss = {| upd := u; unitAnnot := ul; cms := cs; substep := HSubstep |} :: mss)
+      (HCombine: substepsComb (bss ++ css)):
+      SemActionBig (MCall meth (projT1 body) marg cont) (bss ++ css) retv
+  | SABMCassExt
       meth s (marg: Expr type (SyntaxKind (arg s)))
       (mret: type (ret s))
       retK (fret: type retK)
       (cont: type (ret s) -> ActionT type retK)
-      (HNotIn: ~ In meth (getDefs m))
-      newRegs (cs icalls: MethsT) acalls
-      (HNotCalled: ~ M.In meth cs) (* forces no double-call within an action, but necessary *)
-      (HAcalls: acalls = M.add meth (existT _ _ (evalExpr marg, mret)) cs)
-      (HSemAction: SemActionOp (cont mret) newRegs cs icalls fret):
-      SemActionOp (MCall meth s marg cont) newRegs acalls icalls fret
-  | SASMCallInt
-      meth methBody
-      (marg: Expr type (SyntaxKind (arg (projT1 methBody))))
-      (mret: type (ret (projT1 methBody)))
-      retK (fret: type retK)
-      (cont: type (ret (projT1 methBody)) -> ActionT type retK)
-      (HIn: In (meth :: methBody)%struct (getDefsBodies m))
-      cnewRegs ccalls cicalls 
-      (HCallee: SemActionOp ((projT2 methBody) type (evalExpr marg))
-                            cnewRegs ccalls cicalls mret)
-      newRegs (cs icalls: MethsT)
-      (HSemAction: SemActionOp (cont mret) newRegs cs icalls fret)
-      (Hnews: M.Disj cnewRegs newRegs)
-      (Hcalls: M.Disj ccalls cs)
-      (Hicalls: M.Disj cicalls icalls)
-      (Hmethnin1: ~ M.In meth icalls)
-      (Hmethnin2: ~ M.In meth cicalls):
-      SemActionOp (MCall meth (projT1 methBody) marg cont)
-                  (M.union cnewRegs newRegs) (M.union ccalls cs)
-                  (M.union cicalls (M.add meth (existT _ _ (evalExpr marg, mret)) icalls))
-                  fret
-  | SASLet
+      (HNotInDefs: ~ In meth (getDefs m))
+      css retv (HSemActionBig: SemActionBig (cont mret) css retv):
+      SemActionBig (MCall meth s marg cont) css retv
+  | SABLet
       k (e: Expr type k) retK (fret: type retK)
-      (cont: fullType type k -> ActionT type retK) newRegs cs icalls
-      (HSemActionOp: SemActionOp (cont (evalExpr e)) newRegs cs icalls fret):
-      SemActionOp (Let_ e cont) newRegs cs icalls fret
-  | SASReadReg
+      (cont: fullType type k -> ActionT type retK)
+      css retv (HSemActionBig: SemActionBig (cont (evalExpr e)) css retv):
+      SemActionBig (Let_ e cont) css retv
+  | SABReadReg
       (r: string) regT (regV: fullType type regT)
       retK (fret: type retK) (cont: fullType type regT -> ActionT type retK)
-      newRegs cs icalls
-      (HRegVal: M.find r oldRegs = Some (existT _ regT regV))
-      (HSemActionOp: SemActionOp (cont regV) newRegs cs icalls fret):
-      SemActionOp (ReadReg r _ cont) newRegs cs icalls fret
-  | SASWriteReg
+      (HRegVal: M.find r o = Some (existT _ regT regV))
+      css retv (HSemActionBig: SemActionBig (cont regV) css retv):
+      SemActionBig (ReadReg r _ cont) css retv
+  | SABWriteReg
       (r: string) k
       (e: Expr type k)
       retK (fret: type retK)
-      (cont: ActionT type retK) newRegs cs icalls anewRegs
-      (HNotWritten: ~ M.In r newRegs) (* it implies well-formedness *)
-      (HANewRegs: anewRegs = M.add r (existT _ _ (evalExpr e)) newRegs)
-      (HSemActionOp: SemActionOp cont newRegs cs icalls fret):
-      SemActionOp (WriteReg r e cont) anewRegs cs icalls fret
-  | SASIfElseTrue
+      (cont: ActionT type retK)
+      css retv (HSemActionBig: SemActionBig cont css retv):
+      SemActionBig (WriteReg r e cont) css retv
+  | SABIfElseTrue
       (p: Expr type (SyntaxKind Bool)) k1
-      (a: ActionT type k1)
-      (a': ActionT type k1)
-      (r1: type k1)
+      (a a': ActionT type k1)
       k2 (cont: type k1 -> ActionT type k2)
-      newRegs1 newRegs2 calls1 calls2 icalls1 icalls2 (r2: type k2)
       (HTrue: evalExpr p = true)
-      (HAction: SemActionOp a newRegs1 calls1 icalls1 r1)
-      (HSemActionOp: SemActionOp (cont r1) newRegs2 calls2 icalls2 r2)
-      unewRegs ucalls icalls
-      (HUNewRegs: unewRegs = M.union newRegs1 newRegs2)
-      (HregsDisj: M.Disj newRegs1 newRegs2)
-      (HUCalls: ucalls = M.union calls1 calls2)
-      (HcallsDisj: M.Disj calls1 calls2)
-      (Hicalls: icalls = M.union icalls1 icalls2)
-      (HicallsDisj: M.Disj icalls1 icalls2):
-      SemActionOp (IfElse p a a' cont) unewRegs ucalls icalls r2
-  | SASIfElseFalse
+      tss retvt (HAction: SemActionBig a tss retvt)
+      css retv (HSemActionBig: SemActionBig (cont retvt) css retv)
+      (HCombine: substepsComb (tss ++ css)):
+      SemActionBig (IfElse p a a' cont) (tss ++ css) retv
+  | SABIfElseFalse
       (p: Expr type (SyntaxKind Bool)) k1
-      (a: ActionT type k1)
-      (a': ActionT type k1)
-      (r1: type k1)
+      (a a': ActionT type k1)
       k2 (cont: type k1 -> ActionT type k2)
-      newRegs1 newRegs2 calls1 calls2 icalls1 icalls2 (r2: type k2)
-      (HFalse: evalExpr p = false)
-      (HAction: SemActionOp a' newRegs1 calls1 icalls1 r1)
-      (HSemActionOp: SemActionOp (cont r1) newRegs2 calls2 icalls2 r2)
-      unewRegs ucalls icalls
-      (HUNewRegs: unewRegs = M.union newRegs1 newRegs2)
-      (HregsDisj: M.Disj newRegs1 newRegs2)
-      (HUCalls: ucalls = M.union calls1 calls2)
-      (HcallsDisj: M.Disj calls1 calls2)
-      (Hicalls: icalls = M.union icalls1 icalls2)
-      (HicallsDisj: M.Disj icalls1 icalls2):
-      SemActionOp (IfElse p a a' cont) unewRegs ucalls icalls r2
-  | SASAssertTrue
+      (HTrue: evalExpr p = false)
+      fss retvf (HAction: SemActionBig a' fss retvf)
+      css retv (HSemActionBig: SemActionBig (cont retvf) fss retv)
+      (HCombine: substepsComb (fss ++ css)):
+      SemActionBig (IfElse p a a' cont) (fss ++ css) retv
+  | SABAssertTrue
       (p: Expr type (SyntaxKind Bool)) k2
-      (cont: ActionT type k2) newRegs2 calls2 icalls2 (r2: type k2)
+      (cont: ActionT type k2)
       (HTrue: evalExpr p = true)
-      (HSemActionOp: SemActionOp cont newRegs2 calls2 icalls2 r2):
-      SemActionOp (Assert_ p cont) newRegs2 calls2 icalls2 r2
-  | SASReturn
-      k (e: Expr type (SyntaxKind k)) evale
-      (HEvalE: evale = evalExpr e):
-      SemActionOp (Return e) (M.empty _) (M.empty _) (M.empty _) evale.
+      css retv (HSemActionBig: SemActionBig cont css retv):
+      SemActionBig (Assert_ p cont) css retv
+  | SABReturn
+      k (e: Expr type (SyntaxKind k)):
+      SemActionBig (Return e) nil (evalExpr e).
 
-  Theorem inversionSemActionOp
-          k a news cs icalls retC
-          (evalA: @SemActionOp k a news cs icalls retC):
-    match a with
-    | MCall meth s e c =>
-      (In meth (getDefs m) /\
-       exists methBody mret cnewRegs ccalls cicalls nnewRegs ncalls nicalls,
-         In (meth :: existT _ s methBody)%struct (getDefsBodies m) /\
-         SemActionOp (methBody type (evalExpr e)) cnewRegs ccalls cicalls mret /\
-         SemActionOp (c mret)
-                     nnewRegs ncalls nicalls retC /\
-         news = M.union cnewRegs nnewRegs /\
-         cs = M.union ccalls ncalls /\
-         icalls = M.union cicalls (M.add meth (existT _ _ (evalExpr e, mret)) nicalls) /\
-         M.Disj cnewRegs nnewRegs /\
-         M.Disj ccalls ncalls /\
-         M.Disj cicalls nicalls /\
-         ~ M.In meth cicalls /\
-         ~ M.In meth nicalls) \/
-      (~ In meth (getDefs m) /\
-       exists mret pcalls,
-         SemActionOp (c mret) news pcalls icalls retC /\
-         ~ M.In meth pcalls /\
-         cs = M.add meth (existT _ _ (evalExpr e, mret)) pcalls)
-    | Let_ _ e cont =>
-      SemActionOp (cont (evalExpr e)) news cs icalls retC
-    | ReadReg r k c =>
-      exists rv,
-      M.find r oldRegs = Some (existT _ k rv) /\
-      SemActionOp (c rv) news cs icalls retC
-    | WriteReg r _ e a =>
-      exists pnews,
-      SemActionOp a pnews cs icalls retC /\
-      ~ M.In r pnews /\
-      news = M.add r (existT _ _ (evalExpr e)) pnews
-    | IfElse p _ aT aF c =>
-      exists news1 calls1 icalls1 news2 calls2 icalls2 r1,
-      match evalExpr p with
-      | true =>
-        SemActionOp aT news1 calls1 icalls1 r1 /\
-        SemActionOp (c r1) news2 calls2 icalls2 retC /\
-        news = M.union news1 news2 /\
-        cs = M.union calls1 calls2 /\
-        icalls = M.union icalls1 icalls2 /\
-        M.Disj icalls1 icalls2
-      | false =>
-        SemActionOp aF news1 calls1 icalls1 r1 /\
-        SemActionOp (c r1) news2 calls2 icalls2 retC /\
-        news = M.union news1 news2 /\
-        cs = M.union calls1 calls2 /\
-        icalls = M.union icalls1 icalls2 /\
-        M.Disj icalls1 icalls2
-      end
-    | Assert_ e c =>
-      SemActionOp c news cs icalls retC /\
-      evalExpr e = true
-    | Return e =>
-      retC = evalExpr e /\
-      news = M.empty _ /\
-      cs = M.empty _ /\
-      icalls = M.empty _
-    end.
-  Proof.
-    destruct evalA; eauto; repeat eexists.
-    - right; repeat eexists; eauto.
-    - left; split.
-      + unfold getDefs, namesOf in *.
-        replace meth with (attrName (meth :: methBody)%struct) by reflexivity.
-        apply in_map; auto.
-      + repeat eexists; eauto.
-        destruct methBody; auto.
-    - destruct (evalExpr p); eauto; try discriminate.
-    - destruct (evalExpr p); eauto; try discriminate.
-  Qed.
+  Inductive SubstepBig: UnitLabel -> list (SubstepRec m o) -> Prop :=
+  | SBRule
+      k (a: Action Void)
+      (HInRules: In {| attrName := k; attrType := a |} (getRules m))
+      u cs (HSubstep: Substep m o u (Rle (Some k)) cs)
+      bss (HActionBig: SemActionBig (a type) bss WO)
+      ss (Hss: ss = {| upd := u; unitAnnot := Rle (Some k);
+                       cms := cs; substep := HSubstep |} :: bss):
+      SubstepBig (Rle (Some k)) ss
+  | SBMeth
+      (f: DefMethT) (HIn: In f (getDefsBodies m))
+      bss marg mret (HActionBig: SemActionBig (projT2 (attrType f) type marg) bss mret)
+      ul (Hul: ul = Meth (Some ((attrName f) :: (existT _ _ (marg, mret)))%struct))
+      u cs (HSubstep: Substep m o u ul cs)
+      ss (Hss: ss = {| upd := u; unitAnnot := ul; cms := cs; substep := HSubstep |} :: bss):
+      SubstepBig ul ss.
 
-  Inductive SubstepOp: UpdatesT -> LabelT -> MethsT ->Prop :=
-  | SSSEmptyRule:
-      forall u l ics,
-        u = M.empty _ ->
-        l = emptyRuleLabel ->
-        ics = M.empty _ ->
-        SubstepOp u l ics
-  | SSSEmptyMeth:
-      forall u l ics,
-        u = M.empty _ ->
-        l = emptyMethLabel ->
-        ics = M.empty _ ->
-        SubstepOp u l ics
-  | SSSRule:
-      forall k (a: Action Void)
-             (HInRules: List.In {| attrName := k; attrType := a |} (getRules m))
-             u cs ics (HAction: SemActionOp (a type) u cs ics WO) ndefs,
-        ndefs = M.empty _ ->
-        SubstepOp u {| annot := Some (Some k);
-                       defs := ndefs;
-                       calls := cs |} ics
-  | SSSMeth:
-      forall (f: DefMethT)
-             (HIn: In f (getDefsBodies m))
-             (HNotIn: ~ In (attrName f) (getCalls m))
-             u cs ics argV retV
-             (HAction: SemActionOp ((projT2 (attrType f)) type argV) u cs ics retV)
-             adefs,
-        adefs = M.add (attrName f) (existT _ _ (argV, retV)) (M.empty _) ->
-        SubstepOp u {| annot := None;
-                       defs := adefs;
-                       calls := cs |} ics.
+  Inductive SubstepsBig: list UnitLabel -> list (SubstepRec m o) -> Prop :=
+  | SSBNil: SubstepsBig nil nil
+  | SSBCons
+      ull sss (Hss: SubstepsBig ull sss)
+      ul ss (Hs: SubstepBig ul ss)
+      (HCombine: substepsComb (ss ++ sss)):
+      SubstepsBig (ul :: ull) (ss ++ sss).
 
-  Inductive SubstepsOp: UpdatesT -> LabelT -> MethsT -> Prop :=
-  | SSSNil:
-      SubstepsOp (M.empty _) emptyMethLabel (M.empty _)
-  | SSSCons:
-      forall pu pl pics,
-        SubstepsOp pu pl pics ->
-        forall nu nl nics,
-          CanCombineUL pu nu pl nl ->
-          M.Disj pics nics ->
-          SubstepOp nu nl nics ->
-          SubstepsOp (M.union pu nu) (mergeLabel pl nl) (M.union pics nics).
+  Inductive StepBig: list UnitLabel -> UpdatesT -> LabelT -> Prop :=
+  | StepIntro
+      ull sss (HSubsteps: SubstepsBig ull sss)
+      u (Hu: u = foldSSUpds sss)
+      l (Hl: l = hide (foldSSLabel sss)):
+      StepBig ull u l.
 
-  Inductive StepOp: UpdatesT -> LabelT -> Prop :=
-  | StepOpIntro: forall u l ics (HSubSteps: SubstepsOp u l ics),
-      StepOp u l.
-
-End GivenModule.
-
-Ltac invertActionOp H := apply inversionSemActionOp in H; simpl in H; dest; try subst.
-Ltac invertActionOpFirst :=
-  match goal with
-  | [H: SemActionOp _ _ _ _ _ _ _ |- _] => invertActionOp H
-  end.
-Ltac invertActionOpRep :=
-  repeat
-    match goal with
-    | [H: SemActionOp _ _ _ _ _ _ _ |- _] => invertActionOp H
-    | [H: if ?c
-          then
-            SemActionOp _ _ _ _ _ _ _ /\ _ /\ _ /\ _
-          else
-            SemActionOp _ _ _ _ _ _ _ /\ _ /\ _ /\ _ |- _] =>
-      let ic := fresh "ic" in
-      (remember c as ic; destruct ic; dest; subst)
+  Definition toUnitLabelsD (meths: MethsT) :=
+    M.fold (fun m ar l => (Meth (Some (m :: ar)%struct)) :: l)
+           meths nil.
+  
+  Definition toUnitLabels (l: LabelT) :=
+    match annot l with
+    | Some (Some s) => Rle (Some s) :: (toUnitLabelsD (defs l))
+    | _ => toUnitLabelsD (defs l)
     end.
 
-Section Facts.
+End BigSem.
+
+Section Relaxed.
   Variable m: Modules.
-
-  Lemma semActionOp_icalls:
-    forall o {retK} (a: ActionT type retK) u cs ics retv,
-      SemActionOp m o a u cs ics retv ->
-      M.KeysSubset ics (getDefs m).
-  Proof.
-    induction 1; simpl; intros; subst; auto.
-    - apply M.KeysSubset_union; auto.
-      apply M.KeysSubset_add; auto.
-      unfold getDefs, namesOf.
-      induction (getDefsBodies m).
-      + intuition.
-      + simpl in *.
-        destruct HIn; subst.
-        * intuition.
-        * specialize (IHl H1).
-          intuition.
-    - apply M.KeysSubset_union; auto.
-    - apply M.KeysSubset_union; auto.
-    - apply M.KeysSubset_empty; auto.
-  Qed.
-
-  Lemma semActionOp_calls:
-    forall o {retK} (a: ActionT type retK) u cs ics retv,
-      SemActionOp m o a u cs ics retv ->
-      M.KeysDisj cs (getDefs m).
-  Proof.
-    induction 1; simpl; intros; subst; auto.
-    - apply M.KeysDisj_add; auto.
-    - apply M.KeysDisj_union; auto.
-    - apply M.KeysDisj_union; auto.
-    - apply M.KeysDisj_union; auto.
-    - apply M.KeysDisj_empty.
-  Qed.
-
-  Lemma substepOp_calls:
-    forall o u l ics,
-      SubstepOp m o u l ics ->
-      M.KeysDisj (calls l) (getDefs m).
-  Proof.
-    induction 1; simpl; subst; intros.
-    - apply M.KeysDisj_empty.
-    - apply M.KeysDisj_empty.
-    - eapply semActionOp_calls; exact HAction.
-    - eapply semActionOp_calls; exact HAction.
-  Qed.
-
-  Lemma substepsOp_calls:
-    forall o u l ics,
-      SubstepsOp m o u l ics ->
-      M.KeysDisj (calls l) (getDefs m).
-  Proof.
-    induction 1; simpl; intros.
-    - apply M.KeysDisj_empty.
-    - apply substepOp_calls in H2.
-      destruct nl, pl; simpl in *.
-      apply M.KeysDisj_union; auto.
-  Qed.
-
-  Lemma stepOp_calls:
-    forall o u l,
-      StepOp m o u l ->
-      M.KeysDisj (calls l) (getDefs m).
-  Proof. induction 1; eapply substepsOp_calls; eauto. Qed.
-
-End Facts.
-
-Require Import Wf Program.Equality StaticDynamic Equiv.
-
-Section Consistency.
-  Variable m: Modules.
-  Hypothesis (Hwfm: WfModules type m).
-  Variable mEquiv: ModEquiv type typeUT m.
   Variable o: RegsT.
 
-  Lemma SemActionOp_implies_SemActionSubsteps:
-    forall k (a: ActionT type k) u ecs ics retv,
-      SemActionOp m o a u ecs ics retv ->
-      exists u1 cs1 u2 l2,
-        SemAction o a u1 cs1 retv /\
-        SubstepsInd m o u2 l2 /\
-        M.Disj u1 u2 /\
-        M.Disj cs1 (calls l2) /\
-        u = M.union u1 u2 /\
-        (forall k v, M.MapsTo k v ics <-> (M.MapsTo k v cs1 \/ M.MapsTo k v (calls l2)) /\
-                                          (M.MapsTo k v (defs l2))) /\
-        (forall k v, M.MapsTo k v ecs <-> (M.MapsTo k v cs1 \/ M.MapsTo k v (calls l2)) /\
-                                          ~ (M.In k (defs l2))).
-  Proof.
-    intros ? ? ? ? ? ? so.
-    dependent induction so; subst; dest.
-    - exists x.
-      exists (M.add meth (existT _ _ (evalExpr marg, mret)) x0).
-      exists x1.
-      exists x2.
-      intuition.
-      + econstructor; eauto.
-      + apply M.Disj_add_1; try assumption.
-        unfold not; intros.
-        apply M.MapsToIn2 in H6; dest.
-        specialize (H5 meth x3).
-        destruct H5.
-        assert (sth: M.In meth (defs x2) -> False).
-        { intros.
-          apply staticDynDefsSubstepsInd with (x := meth) in H0.
-          intuition.
-          intuition.
-        }
-        assert (sth2: M.MapsTo meth x3 cs) by intuition.
-        apply M.MapsToIn1 in sth2.
-        intuition.
-      + specialize (H4 k v); specialize (H5 k v).
-        apply H4 in H6.
-        dest.
-        destruct H6; [ left | right; assumption].
-        apply M.F.P.F.add_mapsto_iff; try assumption.
-        destruct (string_dec meth k); subst; [left | right; intuition].
-        constructor;
-        try reflexivity.
-        assert (sth: M.MapsTo k v icalls) by intuition.
-        apply semActionOp_icalls in so.
-        apply M.MapsToIn1 in sth.
-        specialize (so _ sth).
-        intuition.
-      + apply H4 in H6; dest.
-        intuition.
-      + apply M.F.P.F.add_mapsto_iff in H6.
-        destruct H6; dest.
-        * subst.
-          apply M.MapsToIn1 in H8.
-          apply staticDynDefsSubstepsInd with (x := k) in H0.
-          intuition.
-          intuition.
-        * specialize (H4 k v); intuition.
-      + specialize (H4 k v); intuition.
-      + apply M.F.P.F.add_mapsto_iff in H6.
-        destruct H6; dest; subst.
-        left; apply M.F.P.F.add_mapsto_iff; intuition.
-        apply H5 in H7; dest.
-        destruct H3; try assumption.
-        left.
-        apply M.F.P.F.add_mapsto_iff.
-        right; intuition.
-        intuition.
-      + apply M.F.P.F.add_mapsto_iff in H6; destruct H6; dest; subst.
-        apply staticDynDefsSubstepsInd with (x := k) in H0; intuition.
-        apply H5 in H8; intuition.
-      + apply M.F.P.F.add_mapsto_iff.
-        apply M.F.P.F.add_mapsto_iff in H6.
-        destruct H6; [left | right]; intuition.
-        specialize (H5 k v); intuition.
-      + apply M.F.P.F.add_mapsto_iff.
-        assert (sth: M.MapsTo k v cs) by (specialize (H5 k v); intuition).
-        destruct (string_dec meth k); subst; [left | right]; intuition.
-        apply M.MapsToIn1 in sth.
-        intuition.
-    - admit.
-    - exists x; exists x0; exists x1; exists x2.
-      intuition.
-      econstructor; eauto.
-    - exists x; exists x0; exists x1; exists x2.
-      intuition.
-      econstructor; eauto.
-    - exists (M.add r (existT _ _ (evalExpr e)) x).
-      exists x0.
-      exists x1; exists x2.
-      intuition.
-      + econstructor; eauto.
-      + subst; dest_disj; solve_disj.
-        unfold not; intros.
-        admit.
-      + admit.
-    - exists (M.union x3 x).
-      exists (M.union x4 x0).
-      exists (M.union x5 x1).
-      exists (mergeLabel x6 x2).
-      intuition.
-      + econstructor; eauto.
-      + admit.
-      + subst.
-        dest_disj.
-        solve_disj.
-      + admit.
-      + subst; meq.
-      + apply M.mapsto_union in H13; dest.
-        unfold mergeLabel; destruct x6, x2; simpl.
-        destruct H13; dest.
-        * apply H11 in H13; simpl in *; dest.
-          { destruct H13.
-            - left; apply M.mapsto_union; auto.
-            - right; apply M.mapsto_union; auto.
-          }
-        * apply H4 in H14; simpl in *; dest.
-          { destruct H14.
-            - left; apply M.mapsto_union.
-              right; constructor; unfold not; intros; auto.
-              admit.
-            - right; apply M.mapsto_union.
-              right; constructor; unfold not; intros; auto.
-              admit.
-          } 
-              
-      + admit.
-      + admit.
-      + admit.
-      + admit.
-      + admit.
-      + admit.
-      + admit.
-    - admit.
-    - exists x; exists x0; exists x1; exists x2.
-      intuition.
-      econstructor; eauto.
-    - repeat (econstructor; eauto); intros; simpl in *; dest.
-      apply M.F.P.F.empty_mapsto_iff in H0; intuition.
-      apply M.F.P.F.empty_mapsto_iff in H; intuition.
-      destruct H;
-        apply M.F.P.F.empty_mapsto_iff in H; intuition.
-  Qed.
+  Inductive SemActionRelaxed:
+    forall k, ActionT type k -> list (SubstepRec m o) -> type k -> Prop :=
+  | SARMCassInt
+      meth body
+      (marg: Expr type (SyntaxKind (arg (projT1 body))))
+      (mret: type (ret (projT1 body)))
+      retK (fret: type retK)
+      (cont: type (ret (projT1 body)) -> ActionT type retK)
+      (HIn: In (meth :: body)%struct (getDefsBodies m))
+      css retv (HCont: SemActionRelaxed (cont mret) css retv)
+      mss (HRelaxed: SemActionRelaxed (projT2 body type (evalExpr marg)) mss mret)
+      ul (Hul: ul = Meth (Some (meth :: (existT _ _ (evalExpr marg, mret)))%struct))
+      u cs (HSubstep: Substep m o u ul cs)
+      bss (Hbss: bss = {| upd := u; unitAnnot := ul; cms := cs; substep := HSubstep |} :: mss)
+      (HCombine: substepsComb (bss ++ css)):
+      SemActionRelaxed (MCall meth (projT1 body) marg cont) (bss ++ css) retv
+  | SARMCassExt
+      meth s (marg: Expr type (SyntaxKind (arg s)))
+      (mret: type (ret s))
+      retK (fret: type retK)
+      (cont: type (ret s) -> ActionT type retK)
+      (* (HNotInDefs: ~ In meth (getDefs m)) *) (* a relaxed point *)
+      css retv (HSemActionRelaxed: SemActionRelaxed (cont mret) css retv):
+      SemActionRelaxed (MCall meth s marg cont) css retv
+  | SARLet
+      k (e: Expr type k) retK (fret: type retK)
+      (cont: fullType type k -> ActionT type retK)
+      css retv (HSemActionRelaxed: SemActionRelaxed (cont (evalExpr e)) css retv):
+      SemActionRelaxed (Let_ e cont) css retv
+  | SARReadReg
+      (r: string) regT (regV: fullType type regT)
+      retK (fret: type retK) (cont: fullType type regT -> ActionT type retK)
+      (HRegVal: M.find r o = Some (existT _ regT regV))
+      css retv (HSemActionRelaxed: SemActionRelaxed (cont regV) css retv):
+      SemActionRelaxed (ReadReg r _ cont) css retv
+  | SARWriteReg
+      (r: string) k
+      (e: Expr type k)
+      retK (fret: type retK)
+      (cont: ActionT type retK)
+      css retv (HSemActionRelaxed: SemActionRelaxed cont css retv):
+      SemActionRelaxed (WriteReg r e cont) css retv
+  | SARIfElseTrue
+      (p: Expr type (SyntaxKind Bool)) k1
+      (a a': ActionT type k1)
+      k2 (cont: type k1 -> ActionT type k2)
+      (HTrue: evalExpr p = true)
+      tss retvt (HAction: SemActionRelaxed a tss retvt)
+      css retv (HSemActionRelaxed: SemActionRelaxed (cont retvt) css retv)
+      (HCombine: substepsComb (tss ++ css)):
+      SemActionRelaxed (IfElse p a a' cont) (tss ++ css) retv
+  | SARIfElseFalse
+      (p: Expr type (SyntaxKind Bool)) k1
+      (a a': ActionT type k1)
+      k2 (cont: type k1 -> ActionT type k2)
+      (HTrue: evalExpr p = false)
+      fss retvf (HAction: SemActionRelaxed a' fss retvf)
+      css retv (HSemActionRelaxed: SemActionRelaxed (cont retvf) fss retv)
+      (HCombine: substepsComb (fss ++ css)):
+      SemActionRelaxed (IfElse p a a' cont) (fss ++ css) retv
+  | SARAssertTrue
+      (p: Expr type (SyntaxKind Bool)) k2
+      (cont: ActionT type k2)
+      (HTrue: evalExpr p = true)
+      css retv (HSemActionRelaxed: SemActionRelaxed cont css retv):
+      SemActionRelaxed (Assert_ p cont) css retv
+  | SARReturn
+      k (e: Expr type (SyntaxKind k)):
+      SemActionRelaxed (Return e) nil (evalExpr e).
 
-  Lemma step_implies_StepOp:
-    forall o u l,
-      Step m o u l -> StepOp m o u l.
+  Inductive SubstepRelaxed: UnitLabel -> list (SubstepRec m o) -> Prop :=
+  | SRRule
+      k (a: Action Void)
+      (HInRules: In {| attrName := k; attrType := a |} (getRules m))
+      u cs (HSubstep: Substep m o u (Rle (Some k)) cs)
+      bss (HActionRelaxed: SemActionRelaxed (a type) bss WO)
+      ss (Hss: ss = {| upd := u; unitAnnot := Rle (Some k);
+                       cms := cs; substep := HSubstep |} :: bss):
+      SubstepRelaxed (Rle (Some k)) ss
+  | SRMeth
+      (f: DefMethT) (HIn: In f (getDefsBodies m))
+      bss marg mret (HActionRelaxed: SemActionRelaxed (projT2 (attrType f) type marg) bss mret)
+      ul (Hul: ul = Meth (Some ((attrName f) :: (existT _ _ (marg, mret)))%struct))
+      u cs (HSubstep: Substep m o u ul cs)
+      ss (Hss: ss = {| upd := u; unitAnnot := ul; cms := cs; substep := HSubstep |} :: bss):
+      SubstepRelaxed ul ss.
+
+  Inductive SubstepsRelaxed: list UnitLabel -> list (SubstepRec m o) -> Prop :=
+  | SSRNil: SubstepsRelaxed nil nil
+  | SSRCons
+      ull sss (Hss: SubstepsRelaxed ull sss)
+      ul ss (Hs: SubstepRelaxed ul ss)
+      (HCombine: substepsComb (ss ++ sss)):
+      SubstepsRelaxed (ul :: ull) (ss ++ sss).
+
+  Inductive StepRelaxed: list UnitLabel -> UpdatesT -> LabelT -> Prop :=
+  | StepRIntro
+      ull sss (HSubsteps: SubstepsRelaxed ull sss)
+      u (Hu: u = foldSSUpds sss)
+      l (Hl: l = hide (foldSSLabel sss)):
+      StepRelaxed ull u l.
+
+End Relaxed.
+
+Section Consistency.
+
+  Lemma substeps_implies_stepRelaxed:
+    forall m o (ss: Substeps m o),
+      substepsComb ss ->
+      SubstepsRelaxed (toUnitLabels (hide (foldSSLabel ss))) ss.
   Proof.
     admit.
   Qed.
+
+  Lemma relaxed_to_big:
+    forall m o (ss: Substeps m o) ull,
+      SubstepsRelaxed ull ss ->
+      wellHidden m (hide (foldSSLabel ss)) ->
+      SubstepsBig ull ss.
+  Proof.
+    admit.
+  Qed.
+
+  Lemma step_implies_StepBig:
+    forall m o u l,
+      Step m o u l ->
+      (* TODO: need a nocycle condition *)
+      StepBig m o (toUnitLabels l) u l.
+  Proof.
+    intros; inv H.
+    econstructor; eauto.
+    apply relaxed_to_big; auto.
+    apply substeps_implies_stepRelaxed; auto.
+  Qed.
+
+  (* Lemma decomposition_big: *)
+  (*   forall m o *)
+  (*          (Hss: forall ul (ss: list (SubstepRec m o)), *)
+  (*              SubstepBig ul ss -> *)
+  (*              Step m o (foldSSUpds ss) (hide (mergeLabel (getLabel ul (M.empty _)) *)
+  (*                                                         (foldSSLabel ss)))) *)
+  (*          ull u l *)
+  (*          (HStepBig: StepBig m o ull u l), *)
+  (*     Step m o u l. *)
+  (* Proof. *)
     
 End Consistency.
 
